isabelle/core/MergeSubsts.thy
@@ -1,0 +1,183 @@
+theory MergeSubsts
+  imports MergeSubstsHelpers LinkError
+begin
+
+(* The merge_substs operation to merge two type substitutions. *)
+
+(* The problem being solved here is that when linking CoreModules, we need to merge 
+   their CM_TypeSubsts (abstract type definitions).
+
+   For example, if module 1 defines "type A = B;" and module 2 defines "type B = i32;",
+   we need to merge these to get a new type substitution [A := i32, B := i32] in which
+   each type is fully resolved.
+
+   Below, we define "merge_substs" which accomplishes this. If merge_substs s1 s2
+   returns Inr \<sigma>, then \<sigma> is the unique idempotent closure of the union of s1 and s2 (see
+   is_subst_closure, defined in MergeSubstPrelims.thy). Otherwise, either s1 and s2 are
+   inconsistent (map the same abstract type T to different concrete realizations - which
+   can't happen if the input modules were built from the same source program), or there
+   is a dependency cycle (which is a user error).
+
+   merge_substs is a non-executable specification only; the "merge_all_substs" function
+   (defined elsewhere) provides an executable version.
+
+   We also prove some properties, e.g. merge_substs is associative, commutative,
+   idempotent (merging a subst with itself returns the same subst), and the
+   empty subst is an identity (merging with the empty subst has no effect).
+*)
+
+
+(* ========================================================================== *)
+(* Definition of merge_substs *)
+(* ========================================================================== *)
+
+(* The union of two substitutions is well-defined (order-immaterial) when they
+   are consistent. We take the right-biased ++f as the canonical representative. *)
+abbreviation subst_union :: "TypeSubst \<Rightarrow> TypeSubst \<Rightarrow> TypeSubst" where
+  "subst_union s1 s2 \<equiv> s1 ++\<^sub>f s2"
+
+(* Given a substitution u satisfying acyclic_subst_deps u, there exists a
+   unique substitution \<sigma> satisfying is_subst_closure u \<sigma>. *)
+(* See also: MergeSubstPrelims.thy for definition of is_subst_closure, and
+   MergeSubstHelpers.thy for proofs. *)
+lemma subst_closure_exists_unique:
+  assumes "acyclic_subst_deps u"
+  shows "\<exists>!\<sigma>. is_subst_closure u \<sigma>"
+  using assms resolve_subst_is_closure subst_closure_unique by auto
+
+(* merge_substs s1 s2:
+   - LinkConflict if s1 and s2 disagree on a shared abstract type;
+   - LinkCycle if the equation set's dependency relation is cyclic (no unique
+     idempotent closure);
+   - otherwise the (unique) idempotent closure of the union of the two equation
+     sets.
+  The use of THE is justified by subst_closure_exists_unique. *)
+definition merge_substs :: "TypeSubst \<Rightarrow> TypeSubst \<Rightarrow> (LinkError, TypeSubst) sum" where
+  "merge_substs s1 s2 =
+     (if \<not> consistent_subst s1 s2 then Inl LinkConflict
+      else if \<not> acyclic_subst_deps (subst_union s1 s2) then Inl LinkCycle
+      else Inr (THE \<sigma>. is_subst_closure (subst_union s1 s2) \<sigma>))"
+
+(* merge_substs s1 s2 is Inr \<sigma> exactly when s1,s2 are consistent, have acyclic union,
+   and \<sigma> is the (unique) idempotent closure of their union. *)
+lemma merge_substs_eq_Inr_iff:
+  "merge_substs s1 s2 = Inr \<sigma> \<longleftrightarrow>
+     consistent_subst s1 s2 \<and> acyclic_subst_deps (subst_union s1 s2)
+       \<and> is_subst_closure (subst_union s1 s2) \<sigma>"
+proof
+  assume "merge_substs s1 s2 = Inr \<sigma>"
+  then have cons: "consistent_subst s1 s2"
+        and acyc: "acyclic_subst_deps (subst_union s1 s2)"
+        and the_eq: "(THE \<sigma>'. is_subst_closure (subst_union s1 s2) \<sigma>') = \<sigma>"
+    unfolding merge_substs_def by (auto split: if_splits)
+  have "is_subst_closure (subst_union s1 s2) \<sigma>"
+    by (metis acyc local.the_eq subst_closure_exists_unique the_equality)
+  thus "consistent_subst s1 s2
+      \<and> acyclic_subst_deps (subst_union s1 s2)
+      \<and> is_subst_closure (subst_union s1 s2) \<sigma>" using acyc cons by simp
+next
+  assume "consistent_subst s1 s2 \<and> acyclic_subst_deps (subst_union s1 s2)
+            \<and> is_subst_closure (subst_union s1 s2) \<sigma>"
+  thus "merge_substs s1 s2 = Inr \<sigma>"
+    using merge_substs_def subst_closure_exists_unique the_equality
+    by metis
+qed
+
+
+(* ========================================================================== *)
+(* Algebraic laws                                                             *)
+(* ========================================================================== *)
+
+(* merge_substs is commutative *)
+lemma merge_substs_commute:
+  "merge_substs s1 s2 = merge_substs s2 s1"
+proof (cases "consistent_subst s1 s2")
+  case False
+  then have "\<not> consistent_subst s2 s1" by (simp add: consistent_subst_sym)
+  with False show ?thesis unfolding merge_substs_def by simp
+next
+  case True
+  then have cons2: "consistent_subst s2 s1" by (simp add: consistent_subst_sym)
+  have union_eq: "subst_union s1 s2 = subst_union s2 s1"
+    using consistent_subst_add_commute[OF True] .
+  show ?thesis
+    unfolding merge_substs_def
+    using True cons2 union_eq by simp
+qed
+
+(* fmempty is an identity: merging with the empty substitution returns the
+   other one (when it is idempotent). *)
+lemma merge_substs_empty_left:
+  assumes "idempotent_subst s"
+  shows "merge_substs fmempty s = Inr s"
+proof -
+  have "is_subst_closure (subst_union fmempty s) s"
+    using is_subst_closure_self[OF assms] by simp
+  moreover have "acyclic_subst_deps (subst_union fmempty s)"
+    using idempotent_subst_acyclic[OF assms] by simp
+  ultimately show ?thesis
+    by (simp add: merge_substs_eq_Inr_iff)
+qed
+
+lemma merge_substs_empty_right:
+  assumes "idempotent_subst s"
+  shows "merge_substs s fmempty = Inr s"
+  using merge_substs_empty_left[OF assms] merge_substs_commute by simp
+
+(* Idempotence: merging an idempotent substitution with itself returns it. *)
+lemma merge_substs_idem:
+  assumes "idempotent_subst s"
+  shows "merge_substs s s = Inr s"
+proof -
+  have "is_subst_closure (subst_union s s) s"
+    using is_subst_closure_self[OF assms] by simp
+  moreover have "acyclic_subst_deps (subst_union s s)"
+    using idempotent_subst_acyclic[OF assms] by simp
+  moreover have "consistent_subst s s"
+    unfolding consistent_subst_def by simp
+  ultimately show ?thesis
+    using merge_substs_eq_Inr_iff by simp
+qed
+
+(* merge_substs is associative (when linking succeeds). *)
+lemma merge_substs_assoc:
+  assumes ab:    "merge_substs s1 s2 = Inr a"
+      and bc:    "merge_substs s2 s3 = Inr b"
+      and r:     "merge_substs a s3 = Inr r"
+      and r':    "merge_substs s1 b = Inr r'"
+  shows "r = r'"
+proof -
+  \<comment> \<open>Unpack the merges we need. \<close>
+  have acyc12: "acyclic_subst_deps (s1 ++\<^sub>f s2)"
+   and cl_a:   "is_subst_closure (s1 ++\<^sub>f s2) a"
+    using ab merge_substs_eq_Inr_iff by auto
+  have cons_a3: "consistent_subst a s3"
+   and acyc_a3: "acyclic_subst_deps (a ++\<^sub>f s3)"
+   and cl_r:    "is_subst_closure (a ++\<^sub>f s3) r"
+    using r merge_substs_eq_Inr_iff by auto
+  have acyc23: "acyclic_subst_deps (s2 ++\<^sub>f s3)"
+   and cl_b:   "is_subst_closure (s2 ++\<^sub>f s3) b"
+    using bc merge_substs_eq_Inr_iff by auto
+  have cl_r':   "is_subst_closure (s1 ++\<^sub>f b) r'"
+    using r' merge_substs_eq_Inr_iff by auto
+
+  \<comment> \<open>The combined raw union is acyclic, recovered from the acyclic a ++f s3. \<close>
+  have acyc: "acyclic_subst_deps ((s1 ++\<^sub>f s2) ++\<^sub>f s3)"
+    using acyclic_subst_deps_transfer[OF acyc12 cons_a3 cl_a acyc_a3] .
+
+  \<comment> \<open>Left side: absorb a back into s1 ++f s2 (a on the left of a ++f s3). \<close>
+  have r_closes: "is_subst_closure ((s1 ++\<^sub>f s2) ++\<^sub>f s3) r"
+    using is_subst_closure_absorb[OF acyc12 cons_a3 cl_a cl_r] .
+
+  \<comment> \<open>Right side: absorb b back into s2 ++f s3 (b on the right of s1 ++f b). No
+      consistency or commuting needed. \<close>
+  have r'_closes: "is_subst_closure (s1 ++\<^sub>f (s2 ++\<^sub>f s3)) r'"
+    using is_subst_closure_absorb_right[OF acyc23 cl_b cl_r'] .
+
+  \<comment> \<open>Both r and r' close the same acyclic raw union; conclude by uniqueness. \<close>
+  have "is_subst_closure ((s1 ++\<^sub>f s2) ++\<^sub>f s3) r'"
+    using r'_closes by simp
+  with subst_closure_unique[OF acyc r_closes] show "r = r'" by blast
+qed
+
+end
